common/ExposedSimulations.v
@@ -399,8 +399,10 @@ Section ExposingMemory.
       split; auto. subst t.
       split; auto.
       eapply inject_incr_trans; eauto.
-      admit. (*inject trace properties*)
-    Admitted.
+      (* apply injtrace_app; auto.
+      apply inject_trace_strong_weak; auto.
+      *)
+      Admitted.
     
     (** *Plus version of simulation*)
     Lemma Injsimulation_plus:
@@ -727,21 +729,7 @@ Section Composition.
     reflexivity.
   Qed.
   
-  Lemma inject_trace_strong_trans:
-    forall f12 f23 t1 t2 t3,
-      inject_trace_strong f12 t1 t2 ->
-      inject_trace_strong f23 t2 t3 ->
-      inject_trace_strong (compose_meminj f12 f23) t1 t3.
-  Proof.
-  Admitted.
 
-  Lemma inject_trace_compose:
-    forall f12 f23 t1 t2 t3,
-      inject_trace f12 t1 t2 ->
-      inject_trace f23 t2 t3 ->
-      inject_trace (compose_meminj f12 f23) t1 t3.
-  Proof.
-  Admitted.
 
   
   Lemma injection_injection_composition:
@@ -831,7 +819,7 @@ Section Composition.
   exists (i2', i1'); exists s3'; exists (compose_meminj f12' f23'), t3'. repeat (split; auto).
   + exists s2',f12', f23'; auto.
   + subst; eapply compose_inject_incr; auto.
-  + subst; eapply inject_trace_strong_trans ; eauto.
+  + subst; eapply inject_trace_strong_compose ; eauto.
   
 - (*match_states preserves at_external *)
   unfold preserves_atx_inj; intros.
@@ -963,7 +951,7 @@ Section Composition.
     * econstructor.
       do 2 eexists.
       repeat split; eauto.
-    * eapply inject_trace_strong_trans; eassumption.
+    * eapply inject_trace_strong_compose; eassumption.
   + intros t' Htrace.
     destruct (inject_trace_strong_interpolation Htrace) as (t2&Htrace12&Htrace23).
     assert (t2 = t2') by (eapply inject_trace_strong_determ; eassumption).
